Update Environments_Contexts folder

theories/Environments_Contexts/REnvironment.v
@@ -1,18 +1,20 @@
 From Coq Require Import Lia Arith.PeanoNat Classical_Prop.
 Require Import Resource Term Cell Evaluation.
-From DeBrLevel Require Import  LevelInterface MapLevelInterface MapLevel MapExtInterface 
-               MapExt.
+From DeBrLevel Require Import MapExtInterface MapExt.
 From MMaps Require Import MMaps.
 
 
 (** * Environment between resources and cells *)
-Module REnvironment <: ShiftValidET.
-Include MapLvlD.MakeShiftValidMapWLLVL Cell.
+Module REnvironment <: EqualityType.
 
-Import Raw Ext.
+Module Raw := MMaps.OrdList.Make Resource.
+Module Ext := MapET Resource Cell Raw.
+
+Include Ext.
+Import Raw OP.P.
 
 (** *** Definition *)
-
+(*
 Definition embeds_func V v := 
     add (new_key V) ([⧐ᵣₓ (new_key V) ≤ 1 ] ⩽ v … ⩾) (shift (new_key V) 1 V).
 
@@ -32,15 +34,16 @@ Definition extracts (V : REnvironment.t) : list (option Λ) :=
                         | Some _ => None
                         | None   => None
                       end) (seq 0 (max_key V)).
+*)
 
-Definition halts (k : Lvl.t) (V : REnvironment.t) := forall (r : resource) (v : 𝑣), 
- find r V = Some v -> halts k (Cell.extract v).
+Definition halts (V : REnvironment.t) := forall (r : resource) (v : 𝑣), 
+ find r V = Some v -> halts (Cell.extract v).
 
 Definition used r (V : REnvironment.t) := exists v, find r V = Some (⩽ … v ⩾).
 Definition unused r (V : REnvironment.t) := exists v, find r V = Some (⩽ v … ⩾).
 
 (** *** Embedding *)
-
+(*
 Lemma embedding_func_new_spec : forall V v,
  new_key (embeds_func_revert v V) = S (new_key V).
 Proof.
@@ -142,158 +145,46 @@ Proof.
     -- now exists λ.
     -- contradiction.
 Qed. 
-
-(** *** Valid *)
-
-
-Lemma valid_wh_spec : forall m v v',
-  valid (new_key m) m -> (new_key m) ⊩ᵣₓ v -> (new_key m) ⊩ᵣₓ v' -> 
-  valid (S (S (new_key m))) (add (S (new_key m)) v (add (new_key m) v' m)).
-Proof.
-  intros. apply valid_add_notin_spec.
-  - rewrite add_in_iff; intro. destruct H2; try lia.
-    apply new_key_notin_spec in H2; auto.
-  - split. 
-    -- unfold Resource.valid; lia.
-    -- split.
-      * apply Cell.valid_weakening with (k := new_key m); auto.
-      * apply valid_add_notin_spec.
-        ** apply new_key_notin_spec; lia.
-        ** split.
-            + unfold Resource.valid; lia.
-            + split.
-              ++ apply Cell.valid_weakening with (k := new_key m); auto.
-              ++ apply valid_weakening with (k := new_key m); auto.
-Qed.
-
-Lemma valid_update_spec : forall m r v k,
-  In r m -> valid k m -> Cell.valid k v -> valid k (add r v m).
-Proof.
-  intro m; induction m using map_induction; intros r v k HIn Hvm Hvv.
-  - unfold Empty in *; exfalso.
-    destruct HIn as [z HM]; now apply (H r z).
-  - rewrite <- valid_Add_spec in Hvm; eauto; destruct Hvm as [Hvx [Hve Hvm]].
-    destruct (Resource.eq_dec x r); subst.
-    -- unfold Add in *; rewrite H0 in *.
-       assert (eq (add r v (add r e m1)) (add r v m1)).
-       { 
-        intro y. destruct (Resource.eq_dec y r); subst.
-        - repeat rewrite add_eq_o; auto.
-        - repeat rewrite add_neq_o; auto.
-       }
-       rewrite H1; clear H1. rewrite valid_add_notin_spec; auto.
-    -- unfold Add in *; rewrite H0 in *. rewrite add_add_2; auto.
-       rewrite valid_add_notin_spec; auto.
-       + repeat split; auto. apply IHm1; auto. apply add_in_iff in HIn.
-          destruct HIn; subst; auto; contradiction.
-       + intro c; apply add_in_iff in c as [c | c]; auto.
-Qed.
-
-#[local] Hint Resolve iff_equiv Equal_equiv logic_eq_equiv  valid_diamond valid_proper
-shift_proper shift_diamond : core.
-
-Lemma valid_in_spec_1 : forall V lb k r,
-  valid lb V -> In r (shift lb k V) <-> In r V.
-Proof.
-  intro V; induction V using map_induction; intros; split; intros.
-  - eapply shift_Empty_iff in H. destruct H1; exfalso; unfold Empty in *.
-    apply (H r x); eauto.
-  - destruct H1; unfold Empty in *; exfalso; now apply (H r x).
-  - unfold Add in *; rewrite H0 in *. 
-    apply valid_add_notin_spec in H1 as [Hvk [Hvd Hv]]; auto.
-    rewrite shift_add_notin_spec in H2; auto.
-    rewrite add_in_iff in *; destruct H2 as [Heq | HIn]; subst.
-    -- left; rewrite Resource.shift_valid_refl; auto.
-    -- right. rewrite <- IHV1; eauto.
-  - unfold Add in *; rewrite H0 in *. 
-    apply valid_add_notin_spec in H1 as [Hvk [Hvd Hv]]; auto.
-    rewrite shift_add_notin_spec; auto.
-    rewrite add_in_iff in *; destruct H2 as [Heq | HIn]; subst.
-    -- left; rewrite Resource.shift_valid_refl; auto.
-    -- right. rewrite IHV1; eauto.
-Qed.
-
-(** *** Shift *)
-
-Lemma shift_new_in_spec : forall r V,
-  In r V ->  r < new_key V.
-Proof.
-  intros r V; revert r; induction V using map_induction; intros.
-  - exfalso; destruct H0; unfold Empty in H; now apply (H r x).
-  - apply new_key_Add_spec in H0 as H0'; eauto. destruct H0' as [[Heq Hlt] | [Heq Hgt]]; subst.
-    -- rewrite Heq. unfold Add in H0; rewrite H0 in *.
-       rewrite add_in_iff in H1; destruct H1; subst; try lia.
-       apply IHV1 in H1; lia.
-    -- rewrite Heq. unfold Add in H0; rewrite H0 in *.
-       rewrite add_in_iff in H1; destruct H1; subst; try lia.
-       apply IHV1 in H1; lia.
-Qed. 
-
-
-Lemma shift_in_e_spec : forall lb k r V,
-  In r (shift lb k V) -> exists r', r =  ([⧐ᵣ lb ≤ k] r').
-Proof.
-  intros lb k r V; revert lb k r; induction V using map_induction; intros.
-  - eapply shift_Empty_iff in H. unfold Empty in *; exfalso.
-    destruct H0; apply (H r x); eauto.
-  - apply shift_Add_spec_1 with (lb := lb) (k := k) in H0 as H0'; auto.
-    unfold Add in H0'. rewrite H0' in H1; clear H0'.
-    rewrite add_in_iff in H1; destruct H1; subst.
-    -- now exists x.
-    -- auto.
-Qed.
+*)
 
 (** *** Halts *)
 
-Lemma halts_add_spec : forall m k x v,
-  (Evaluation.halts k (Cell.extract v)) /\ halts k m -> halts k (add x v m).
+Lemma halts_add_spec : forall m x v,
+  (Evaluation.halts (Cell.extract v)) /\ halts m -> halts (add x v m).
 Proof.
-  intros m k x v [Hltv Hltm]; unfold halts; intros r v' Hfi.
-  rewrite add_o in Hfi; destruct (Resource.eq_dec x r); subst; inversion Hfi; subst; auto.
+  intros m x v [Hltv Hltm]; unfold halts; intros r v' Hfi.
+  rewrite OP.P.add_o in Hfi; destruct (Resource.eq_dec x r); subst; inversion Hfi; subst; auto.
   apply Hltm in Hfi; auto.
-Qed.
-
-(*
-Lemma halts_valid_weakening : forall V k k',
-  k <= k' -> halts k V -> halts k' (shift k (k' - k) V).
-Proof.
- unfold halts; intros V k k' Hlt Hhlt r v Hfi.
-*)
-
-Lemma max_key_wh_spec : forall (m : t) v v',
-  max_key (add (S (S (max_key m))) v (add (S (max_key m)) v' m)) = S (S (max_key m)).
-Proof.
-  intros. assert (~In (S (max_key m)) m) by (apply max_key_notin_spec; lia).
-  assert (~In (S (S (max_key m))) (add (S (max_key m)) v' m)).
-  - apply max_key_notin_spec. rewrite max_key_add_spec_1; auto; lia.
-  - rewrite max_key_add_spec_1; auto. rewrite max_key_add_spec_1; auto.
 Qed.
 
 (** *** Morphism *)
 
 #[global] 
 Instance in_renv : 
-  Proper (Logic.eq ==> eq ==> iff) In.
+  Proper (Logic.eq ==> REnvironment.eq ==> iff) In.
 Proof.
   repeat red; intros; split; intros;
-  apply Equal_Eqdom in H0; eapply In_m in H0; eauto;
+  apply OP.P.Equal_Eqdom in H0; eapply OP.P.In_m in H0; eauto;
   apply H0; eauto. 
 Qed.
 
 #[global] 
-Instance find_renv : Proper (Logic.eq ==> eq ==> Logic.eq) find.
+Instance find_renv : Proper (Logic.eq ==> REnvironment.eq ==> Logic.eq) find.
 Proof. repeat red; intros; subst. now rewrite H0. Qed.
 
 #[global] 
-Instance Empty_renv : Proper (eq ==> iff) Empty.
+Instance Empty_renv : Proper (REnvironment.eq ==> iff) OP.P.Empty.
 Proof. red; red; intros; now apply Empty_eq_spec. Qed.
 
 #[export] 
 Instance Add_renv : 
-Proper (Resource.eq ==> Cell.eq ==> eq ==> eq ==> iff) (@Add Cell.t).
+Proper (Resource.eq ==> Cell.eq ==> REnvironment.eq ==> REnvironment.eq ==> iff) (@OP.P.Add Cell.t).
 Proof. 
-  red; red; red; red; red; intros. apply Cell.eq_leibniz in H0; subst.
-  rewrite H. unfold Add in *. rewrite H1; rewrite H2. split; intros; auto.
+  red; red; red; red; red; intros. apply Cell.eq_leibniz in H0; subst. unfold Resource.eq in H.
+  rewrite H. unfold OP.P.Add in *. split; intros; auto.
+  - unfold Equal in *; intros. rewrite <- H2. rewrite H0. rewrite OP.P.add_m; eauto.
+  - unfold Equal in *; intros. rewrite H2. rewrite H0. rewrite OP.P.add_m; eauto.
+    now symmetry.
 Qed.
 
 #[global] 
@@ -302,18 +193,18 @@ Proper (Resource.eq ==> Cell.eq ==> REnvironment.eq ==> REnvironment.eq)
                                                           (@add Cell.t).
 Proof. 
  red; red; red; red; red; intros; subst; apply Cell.eq_leibniz in H0; subst.
- rewrite H1; now rewrite H. 
+ unfold Equal; intros; rewrite OP.P.add_m; eauto.
 Qed. 
 
 #[global] 
 Instance Submap_env : 
-  Proper (REnvironment.eq ==> REnvironment.eq ==> iff) REnvironment.Submap.
+  Proper (REnvironment.eq ==> REnvironment.eq ==> iff) Submap.
 Proof. 
   repeat red; intros; split; intros.
-  - rewrite REnvironment.Submap_eq_left_spec in H1; eauto.
-    rewrite REnvironment.Submap_eq_right_spec in H1; eauto.
-  - rewrite <- REnvironment.Submap_eq_left_spec in H1; eauto.
-    rewrite <- REnvironment.Submap_eq_right_spec in H1; eauto.
+  - rewrite Submap_eq_left_spec in H1; eauto.
+    rewrite Submap_eq_right_spec in H1; eauto.
+  - rewrite <- Submap_eq_left_spec in H1; eauto.
+    rewrite <- Submap_eq_right_spec in H1; eauto.
 Qed.
 
 End REnvironment.
@@ -331,11 +222,9 @@ Infix "∈ᵣᵦ" := REnvironment.Raw.In (at level 20, no associativity).
 Notation "r '∉ᵣᵦ' Re" := (~ (REnvironment.Raw.In r Re)) (at level 20, 
                                                                         no associativity). 
 Notation "∅ᵣᵦ" := REnvironment.Raw.empty (at level 20, no associativity). 
-Notation "'isEmptyᵣᵦ(' Re ')'" := (REnvironment.Empty Re) (at level 20, no associativity). 
-Notation "'Addᵣᵦ'" := (REnvironment.Add) (at level 20, no associativity). 
+Notation "'isEmptyᵣᵦ(' Re ')'" := (REnvironment.OP.P.Empty Re) (at level 20, no associativity). 
+Notation "'Addᵣᵦ'" := (REnvironment.OP.P.Add) (at level 20, no associativity). 
 Notation "R '⌊' x '⌋ᵣᵦ'"  := (REnvironment.Raw.find x R) (at level 15, x constr).
-Notation "'maxᵣᵦ(' R ')'"  := (REnvironment.Ext.max_key R) (at level 15).
-Notation "'newᵣᵦ(' R ')'"  := (REnvironment.Ext.new_key R) (at level 15).
 Notation "⌈ x ⤆ v '⌉ᵣᵦ' R"  := (REnvironment.Raw.add x v R) (at level 15, 
                                                                           x constr, v constr).
 Notation "R ⌈ x ⩦ v '⌉ᵣᵦ'"  := (REnvironment.Raw.find x R = Some v) (at level 15, 
@@ -346,19 +235,9 @@ Notation "R ⌈ x ⩦ ⊥ '⌉ᵣᵦ'"  := (REnvironment.Raw.find x R = None) (a
 
 Infix "=" := REnvironment.eq : renvironment_scope.
 
-Notation "'[⧐ᵣᵦ' lb '≤' k ']' t" := (REnvironment.shift lb k t) (at level 45, 
-                                                                      right associativity).
-Infix "⊩ᵣᵦ" := REnvironment.valid (at level 20, no associativity).
-
 #[global]
 Instance eq_equiv_re : Equivalence REnvironment.eq.
-Proof. apply REnvironment.Equal_equiv. Qed.
-
-#[global] Instance max_renv : Proper (REnvironment.eq ==> Logic.eq) (REnvironment.Ext.max_key).
-          Proof. apply REnvironment.Ext.max_key_eq. Qed.
-
-#[global] Instance new_renv : Proper (REnvironment.eq ==> Logic.eq) (REnvironment.Ext.new_key).
-          Proof. apply REnvironment.Ext.new_key_eq. Qed.
+Proof. apply REnvironment.OP.P.Equal_equiv. Qed.
 
 #[global] 
 Instance in_renv : 
@@ -371,13 +250,13 @@ Instance find_renv : Proper (Logic.eq ==> REnvironment.eq ==> Logic.eq)
 Proof. apply REnvironment.find_renv. Qed.
 
 #[global] 
-Instance Empty_renv : Proper (REnvironment.eq ==> iff) (REnvironment.Empty).
+Instance Empty_renv : Proper (REnvironment.eq ==> iff) (REnvironment.OP.P.Empty).
 Proof. apply REnvironment.Empty_renv. Qed.
 
 #[global] 
 Instance Add_renv : 
 Proper (Resource.eq ==> Cell.eq ==> REnvironment.eq ==> REnvironment.eq ==> iff) 
-                                                  (@REnvironment.Add Cell.t).
+                                                  (@REnvironment.OP.P.Add Cell.t).
 Proof. apply REnvironment.Add_renv. Qed. 
 
 #[global] 
@@ -394,13 +273,3 @@ Proof. apply REnvironment.Submap_env. Qed.
 #[global] 
 Instance Submap_env_po : PreOrder REnvironment.Submap.
 Proof. apply REnvironment.Submap_po. Qed. 
-
-#[global] 
-Instance valid_renv : Proper (Logic.eq ==> REnvironment.eq ==> iff) REnvironment.valid.
-Proof. apply REnvironment.valid_eq. Qed.
-
-#[global] 
-Instance shift_renv : 
-  Proper (Logic.eq ==> Logic.eq ==> REnvironment.eq ==> REnvironment.eq) REnvironment.shift.
-Proof. apply REnvironment.shift_eq. Qed.
-
